heap2.lean
@@ -1,0 +1,81 @@
+import separation.heap
+
+universes u
+
+noncomputable def part_  (h₀ h₁ : option heap) : option heap :=
+h₀ >>= λ h, h₁ >>= part h
+
+@[simp]
+lemma some_part'
+  (hp₀ hp₁ : heap)
+  (h : hp₀ ## hp₁)
+: some (part' hp₀ hp₁) = part_ (some hp₀) (some hp₁) :=
+by { simp [part_,part,bind,option.bind,dif_pos, h], }
+
+@[simp]
+lemma heap_emp_part_
+  (hp : heap)
+: part_ (some heap.emp) (some hp) = some hp :=
+sorry
+
+@[simp]
+lemma part__heap_emp
+  (hp : heap)
+: part_ (some hp) (some heap.emp) = some hp :=
+sorry
+
+lemma part__assoc
+  (a b c : option heap)
+: part_ (part_ a b) c = part_ a (part_ b c) :=
+sorry
+
+lemma part__comm
+  (a b : option heap)
+: part_ a b = part_ b a :=
+sorry
+
+instance : is_associative (option heap) part_ :=
+⟨ part__assoc ⟩
+instance : is_commutative (option heap) part_ :=
+⟨ part__comm ⟩
+
+lemma disjoint_of_is_some_part_
+  {hp₀ hp₁ : heap}
+  (h : (part_ (some hp₀) (some hp₁)).is_some)
+: hp₀ ## hp₁ :=
+sorry
+
+lemma is_some_of_is_some_part__right
+  (hp₀ : option heap) {hp₁ : option heap}
+  (h : (part_ hp₀ hp₁).is_some)
+: hp₁.is_some :=
+sorry
+
+lemma is_some_of_is_some_part__left
+  {hp₀ : option heap} (hp₁ : option heap)
+  (h : (part_ hp₀ hp₁).is_some)
+: hp₀.is_some :=
+sorry
+
+@[simp]
+lemma some_eq_some_iff (x y : heap)
+: some x = some y ↔ x = y :=
+sorry
+
+def opt_apl : option heap → pointer → option word
+ | (some hp) p := hp p
+ | none _ := none
+
+lemma opt_apl_some (hp : heap) (p : pointer)
+: opt_apl (some hp) p = hp p :=
+rfl
+
+lemma opt_apl_part__maplet (hp : heap) (p : pointer) (v : word)
+  (h : maplet p v ## hp)
+: (opt_apl (part_ (some (maplet p v)) (some hp)) p) = some v :=
+begin
+  simp [part_,has_bind.bind,option.bind],
+  rw [part,dif_pos,opt_apl,part',maplet,if_pos rfl],
+  refl,
+  assumption
+end
